Bignum/Arm/Machine.lean
@@ -3,8 +3,9 @@ Copyright (c) 2025 Alexandre Rademaker. All rights reserved.
 Released under Apache 2.0 license as described in the file LICENSE.
 Author: Alexandre Rademaker
 -/
-module 
+module
 
 public import Bignum.Arm.Machine.State
 public import Bignum.Arm.Machine.Instruction
 public import Bignum.Arm.Machine.Semantics
+public import Bignum.Arm.Machine.Decode
